temp: find_instr_no_overlap

x86/Asm.v
@@ -1141,14 +1141,14 @@ Definition exec_instr (f: function) (i: instruction) (rs: regset) (m: mem) : out
     let addr := Genv.symbol_address ge id Ptrofs.zero in
     match Genv.find_funct ge addr with
     | Some _ =>
-      Next (rs#RA <- (Val.offset_ptr rs#PC Ptrofs.one) #PC <- addr) m
+      Next (rs#RA <- (Val.offset_ptr rs#PC sz) #PC <- addr) m
     | _ => Stuck
     end
   | Pcall_r r sg =>
     let addr := (rs r) in
     match Genv.find_funct ge addr with
     | Some _ =>
-      Next (rs#RA <- (Val.offset_ptr rs#PC Ptrofs.one) #PC <- addr) m
+      Next (rs#RA <- (Val.offset_ptr rs#PC sz) #PC <- addr) m
     | _ => Stuck
     end
   | Pret =>
@@ -1165,14 +1165,14 @@ Definition exec_instr (f: function) (i: instruction) (rs: regset) (m: mem) : out
   (** Pseudo-instructions *)
   | Plabel lbl =>
       Next (nextinstr rs) m
-  | Pallocframe sz ofs_ra ofs_link =>
-    if zle 0 sz then
+  | Pallocframe fsz ofs_ra ofs_link =>
+    if zle 0 fsz then
     match rs # PC with
     |Vptr (Global id) _
      =>
      let (m0,path) := Mem.alloc_frame m id in
-     let (m1, stk) := Mem.alloc m0 0 sz in
-     match Mem.record_frame (Mem.push_stage m1) (Memory.mk_frame sz) with
+     let (m1, stk) := Mem.alloc m0 0 fsz in
+     match Mem.record_frame (Mem.push_stage m1) (Memory.mk_frame fsz) with
      |None => Stuck
      |Some m2 =>
       let sp := Vptr stk Ptrofs.zero in
@@ -1187,8 +1187,8 @@ Definition exec_instr (f: function) (i: instruction) (rs: regset) (m: mem) : out
      end
     |_ => Stuck
     end else Stuck
-  | Pfreeframe sz ofs_ra ofs_link =>
-    if zle 0 sz then
+  | Pfreeframe fsz ofs_ra ofs_link =>
+    if zle 0 fsz then
       match loadvv Mptr m (Val.offset_ptr rs#RSP ofs_ra) with
       | None => Stuck
       | Some ra =>
@@ -1197,10 +1197,10 @@ Definition exec_instr (f: function) (i: instruction) (rs: regset) (m: mem) : out
           | Some sp =>
               match rs#RSP with
               | Vptr stk ofs =>
-                  if check_topframe sz (Mem.astack (Mem.support m)) then
+                  if check_topframe fsz (Mem.astack (Mem.support m)) then
                   if Val.eq sp (parent_sp_stree (Mem.stack (Mem.support m))) then
                   if Val.eq (Vptr stk ofs) (top_sp_stree (Mem.stack (Mem.support m))) then
-                  match Mem.free m stk 0 sz with
+                  match Mem.free m stk 0 fsz with
                   | None => Stuck
                   | Some m' =>
                     match Mem.return_frame m' with
