x86/RealAsm.v
@@ -20,521 +20,9 @@ Require Import SSAsm AsmFacts AsmRegs.
 Section INSTRSIZE.
 Variable instr_size : instruction -> Z.
 
-Fixpoint code_size (c:code) : Z :=
-  match c with
-  |nil => 0
-  |i::c' => code_size c' + instr_size i
-  end.
-
-(** Looking up instructions in a code sequence by position. *)
-
-Fixpoint find_instr (pos: Z) (c: code) {struct c} : option instruction :=
-  match c with
-  | nil => None
-  | i :: il => if zeq pos 0 then Some i else find_instr (pos - instr_size i) il
-  end.
-
-Fixpoint label_pos (lbl: label) (pos: Z) (c: code) {struct c} : option Z :=
-  match c with
-  | nil => None
-  | instr :: c' =>
-    let nextpos := pos + instr_size instr in
-      if is_label lbl instr then Some nextpos else label_pos lbl nextpos c'
-  end.
-
 Section WITHGE.
   Variable ge : Genv.t Asm.fundef unit.
 
-Definition nextinstr (rs: regset) (sz:ptrofs) :=
-  rs#PC <- (Val.offset_ptr rs#PC sz).
-
-Definition nextinstr_nf (rs: regset) (sz:ptrofs) : regset :=
-  nextinstr (undef_regs (CR ZF :: CR CF :: CR PF :: CR SF :: CR OF :: nil) rs) sz.
-
-Definition goto_label (f: function) (lbl: label) (rs: regset) (m: mem) :=
-  match label_pos lbl 0 (fn_code f) with
-  | None => Stuck
-  | Some pos =>
-      match rs#PC with
-      | Vptr b ofs =>
-        match Genv.find_funct_ptr ge b with
-        | Some _ => Next (rs#PC <- (Vptr b (Ptrofs.repr pos))) m
-        | None => Stuck
-        end
-      | _ => Stuck
-    end
-  end.
-
-(** Auxiliaries for memory accesses. *)
-
-Definition exec_load (chunk: memory_chunk) (m: mem)
-                     (a: addrmode) (rs: regset) (rd: preg) (sz:ptrofs):=
-  match Mem.loadv chunk m (eval_addrmode ge a rs) with
-  | Some v => Next (nextinstr_nf (rs#rd <- v) sz) m
-  | None => Stuck
-  end.
-
-Definition exec_store (chunk: memory_chunk) (m: mem)
-                      (a: addrmode) (rs: regset) (r1: preg)
-                      (destroyed: list preg) (sz:ptrofs) :=
-  match Mem.storev chunk m (eval_addrmode ge a rs) (rs r1) with
-  | Some m' => Next (nextinstr_nf (undef_regs destroyed rs) sz) m'
-  | None => Stuck
-  end.
-
-Definition exec_instr_asm (f: function) (i: instruction) (rs: regset) (m: mem) : outcome :=
-  let sz := Ptrofs.repr (instr_size i) in
-  match i with
-  (** Moves *)
-  | Pmov_rr rd r1 =>
-      Next (nextinstr (rs#rd <- (rs r1)) sz) m
-  | Pmovl_ri rd n =>
-      Next (nextinstr_nf (rs#rd <- (Vint n)) sz) m
-  | Pmovq_ri rd n =>
-      Next (nextinstr_nf (rs#rd <- (Vlong n)) sz) m
-  | Pmov_rs rd id =>
-      Next (nextinstr_nf (rs#rd <- (Genv.symbol_address ge id Ptrofs.zero)) sz) m
-  | Pmovl_rm rd a =>
-      exec_load Mint32 m a rs rd sz
-  | Pmovq_rm rd a =>
-      exec_load Mint64 m a rs rd sz
-  | Pmovl_mr a r1 =>
-      exec_store Mint32 m a rs r1 nil sz
-  | Pmovq_mr a r1 =>
-      exec_store Mint64 m a rs r1 nil sz
-  | Pmovsd_ff rd r1 =>
-      Next (nextinstr (rs#rd <- (rs r1)) sz) m
-  | Pmovsd_fi rd n =>
-      Next (nextinstr (rs#rd <- (Vfloat n)) sz) m
-  | Pmovsd_fm rd a =>
-      exec_load Mfloat64 m a rs rd sz
-  | Pmovsd_mf a r1 =>
-      exec_store Mfloat64 m a rs r1 nil sz
-  | Pmovss_fi rd n =>
-      Next (nextinstr (rs#rd <- (Vsingle n)) sz) m
-  | Pmovss_fm rd a =>
-      exec_load Mfloat32 m a rs rd sz
-  | Pmovss_mf a r1 =>
-      exec_store Mfloat32 m a rs r1 nil sz
-  | Pfldl_m a =>
-      exec_load Mfloat64 m a rs ST0 sz
-  | Pfstpl_m a =>
-      exec_store Mfloat64 m a rs ST0 (ST0 :: nil) sz
-  | Pflds_m a =>
-      exec_load Mfloat32 m a rs ST0 sz
-  | Pfstps_m a =>
-      exec_store Mfloat32 m a rs ST0 (ST0 :: nil) sz
-  (** Moves with conversion *)
-  | Pmovb_mr a r1 =>
-      exec_store Mint8unsigned m a rs r1 nil sz
-  | Pmovw_mr a r1 =>
-      exec_store Mint16unsigned m a rs r1 nil sz
-  | Pmovzb_rr rd r1 =>
-      Next (nextinstr (rs#rd <- (Val.zero_ext 8 rs#r1)) sz) m
-  | Pmovzb_rm rd a =>
-      exec_load Mint8unsigned m a rs rd sz
-  | Pmovsb_rr rd r1 =>
-      Next (nextinstr (rs#rd <- (Val.sign_ext 8 rs#r1)) sz) m
-  | Pmovsb_rm rd a =>
-      exec_load Mint8signed m a rs rd sz
-  | Pmovzw_rr rd r1 =>
-      Next (nextinstr (rs#rd <- (Val.zero_ext 16 rs#r1)) sz) m
-  | Pmovzw_rm rd a =>
-      exec_load Mint16unsigned m a rs rd sz
-  | Pmovsw_rr rd r1 =>
-      Next (nextinstr (rs#rd <- (Val.sign_ext 16 rs#r1)) sz) m
-  | Pmovsw_rm rd a =>
-      exec_load Mint16signed m a rs rd sz
-  | Pmovzl_rr rd r1 =>
-      Next (nextinstr (rs#rd <- (Val.longofintu rs#r1)) sz) m
-  | Pmovsl_rr rd r1 =>
-      Next (nextinstr (rs#rd <- (Val.longofint rs#r1)) sz) m
-  | Pmovls_rr rd =>
-      Next (nextinstr (rs#rd <- (Val.loword rs#rd)) sz) m
-  | Pcvtsd2ss_ff rd r1 =>
-      Next (nextinstr (rs#rd <- (Val.singleoffloat rs#r1)) sz) m
-  | Pcvtss2sd_ff rd r1 =>
-      Next (nextinstr (rs#rd <- (Val.floatofsingle rs#r1)) sz) m
-  | Pcvttsd2si_rf rd r1 =>
-      Next (nextinstr (rs#rd <- (Val.maketotal (Val.intoffloat rs#r1))) sz) m
-  | Pcvtsi2sd_fr rd r1 =>
-      Next (nextinstr (rs#rd <- (Val.maketotal (Val.floatofint rs#r1))) sz) m
-  | Pcvttss2si_rf rd r1 =>
-      Next (nextinstr (rs#rd <- (Val.maketotal (Val.intofsingle rs#r1))) sz) m
-  | Pcvtsi2ss_fr rd r1 =>
-      Next (nextinstr (rs#rd <- (Val.maketotal (Val.singleofint rs#r1))) sz) m
-  | Pcvttsd2sl_rf rd r1 =>
-      Next (nextinstr (rs#rd <- (Val.maketotal (Val.longoffloat rs#r1))) sz) m
-  | Pcvtsl2sd_fr rd r1 =>
-      Next (nextinstr (rs#rd <- (Val.maketotal (Val.floatoflong rs#r1))) sz) m
-  | Pcvttss2sl_rf rd r1 =>
-      Next (nextinstr (rs#rd <- (Val.maketotal (Val.longofsingle rs#r1))) sz) m
-  | Pcvtsl2ss_fr rd r1 =>
-      Next (nextinstr (rs#rd <- (Val.maketotal (Val.singleoflong rs#r1))) sz) m
-  (** Integer arithmetic *)
-  | Pleal rd a =>
-      Next (nextinstr (rs#rd <- (eval_addrmode32 ge a rs)) sz) m
-  | Pleaq rd a =>
-      Next (nextinstr (rs#rd <- (eval_addrmode64 ge a rs)) sz) m
-  | Pnegl rd =>
-      Next (nextinstr_nf (rs#rd <- (Val.neg rs#rd)) sz) m
-  | Pnegq rd =>
-      Next (nextinstr_nf (rs#rd <- (Val.negl rs#rd)) sz) m
-  | Paddl_ri rd n =>
-      Next (nextinstr_nf (rs#rd <- (Val.add rs#rd (Vint n))) sz) m
-  | Paddq_ri rd n =>
-      Next (nextinstr_nf (rs#rd <- (Val.addl rs#rd (Vlong n))) sz) m
-  | Psubl_rr rd r1 =>
-      Next (nextinstr_nf (rs#rd <- (Val.sub rs#rd rs#r1)) sz) m
-  | Psubq_rr rd r1 =>
-      Next (nextinstr_nf (rs#rd <- (Val.subl rs#rd rs#r1)) sz) m
-  | Pimull_rr rd r1 =>
-      Next (nextinstr_nf (rs#rd <- (Val.mul rs#rd rs#r1)) sz) m
-  | Pimulq_rr rd r1 =>
-      Next (nextinstr_nf (rs#rd <- (Val.mull rs#rd rs#r1)) sz) m
-  | Pimull_ri rd n =>
-      Next (nextinstr_nf (rs#rd <- (Val.mul rs#rd (Vint n))) sz) m
-  | Pimulq_ri rd n =>
-      Next (nextinstr_nf (rs#rd <- (Val.mull rs#rd (Vlong n))) sz) m
-  | Pimull_r r1 =>
-      Next (nextinstr_nf (rs#RAX <- (Val.mul rs#RAX rs#r1)
-                            #RDX <- (Val.mulhs rs#RAX rs#r1)) sz) m
-  | Pimulq_r r1 =>
-      Next (nextinstr_nf (rs#RAX <- (Val.mull rs#RAX rs#r1)
-                            #RDX <- (Val.mullhs rs#RAX rs#r1)) sz) m
-  | Pmull_r r1 =>
-      Next (nextinstr_nf (rs#RAX <- (Val.mul rs#RAX rs#r1)
-                            #RDX <- (Val.mulhu rs#RAX rs#r1)) sz) m
-  | Pmulq_r r1 =>
-      Next (nextinstr_nf (rs#RAX <- (Val.mull rs#RAX rs#r1)
-                            #RDX <- (Val.mullhu rs#RAX rs#r1)) sz) m
-  | Pcltd =>
-      Next (nextinstr_nf (rs#RDX <- (Val.shr rs#RAX (Vint (Int.repr 31)))) sz) m
-  | Pcqto =>
-      Next (nextinstr_nf (rs#RDX <- (Val.shrl rs#RAX (Vint (Int.repr 63)))) sz) m
-  | Pdivl r1 =>
-      match rs#RDX, rs#RAX, rs#r1 with
-      | Vint nh, Vint nl, Vint d =>
-          match Int.divmodu2 nh nl d with
-          | Some(q, r) => Next (nextinstr_nf (rs#RAX <- (Vint q) #RDX <- (Vint r)) sz) m
-          | None => Stuck
-          end
-      | _, _, _ => Stuck
-      end
-  | Pdivq r1 =>
-      match rs#RDX, rs#RAX, rs#r1 with
-      | Vlong nh, Vlong nl, Vlong d =>
-          match Int64.divmodu2 nh nl d with
-          | Some(q, r) => Next (nextinstr_nf (rs#RAX <- (Vlong q) #RDX <- (Vlong r)) sz) m
-          | None => Stuck
-          end
-      | _, _, _ => Stuck
-      end
-  | Pidivl r1 =>
-      match rs#RDX, rs#RAX, rs#r1 with
-      | Vint nh, Vint nl, Vint d =>
-          match Int.divmods2 nh nl d with
-          | Some(q, r) => Next (nextinstr_nf (rs#RAX <- (Vint q) #RDX <- (Vint r)) sz) m
-          | None => Stuck
-          end
-      | _, _, _ => Stuck
-      end
-  | Pidivq r1 =>
-      match rs#RDX, rs#RAX, rs#r1 with
-      | Vlong nh, Vlong nl, Vlong d =>
-          match Int64.divmods2 nh nl d with
-          | Some(q, r) => Next (nextinstr_nf (rs#RAX <- (Vlong q) #RDX <- (Vlong r)) sz) m
-          | None => Stuck
-          end
-      | _, _, _ => Stuck
-      end
-  | Pandl_rr rd r1 =>
-      Next (nextinstr_nf (rs#rd <- (Val.and rs#rd rs#r1)) sz) m
-  | Pandq_rr rd r1 =>
-      Next (nextinstr_nf (rs#rd <- (Val.andl rs#rd rs#r1)) sz) m
-  | Pandl_ri rd n =>
-      Next (nextinstr_nf (rs#rd <- (Val.and rs#rd (Vint n))) sz) m
-  | Pandq_ri rd n =>
-      Next (nextinstr_nf (rs#rd <- (Val.andl rs#rd (Vlong n))) sz) m
-  | Porl_rr rd r1 =>
-      Next (nextinstr_nf (rs#rd <- (Val.or rs#rd rs#r1)) sz) m
-  | Porq_rr rd r1 =>
-      Next (nextinstr_nf (rs#rd <- (Val.orl rs#rd rs#r1)) sz) m
-  | Porl_ri rd n =>
-      Next (nextinstr_nf (rs#rd <- (Val.or rs#rd (Vint n))) sz) m
-  | Porq_ri rd n =>
-      Next (nextinstr_nf (rs#rd <- (Val.orl rs#rd (Vlong n))) sz) m
-  | Pxorl_r rd =>
-      Next (nextinstr_nf (rs#rd <- Vzero) sz) m
-  | Pxorq_r rd =>
-      Next (nextinstr_nf (rs#rd <- (Vlong Int64.zero)) sz) m
-  | Pxorl_rr rd r1 =>
-      Next (nextinstr_nf (rs#rd <- (Val.xor rs#rd rs#r1)) sz) m
-  | Pxorq_rr rd r1 =>
-      Next (nextinstr_nf (rs#rd <- (Val.xorl rs#rd rs#r1)) sz) m
-  | Pxorl_ri rd n =>
-      Next (nextinstr_nf (rs#rd <- (Val.xor rs#rd (Vint n))) sz) m
-  | Pxorq_ri rd n =>
-      Next (nextinstr_nf (rs#rd <- (Val.xorl rs#rd (Vlong n))) sz) m
-  | Pnotl rd =>
-      Next (nextinstr_nf (rs#rd <- (Val.notint rs#rd)) sz) m
-  | Pnotq rd =>
-      Next (nextinstr_nf (rs#rd <- (Val.notl rs#rd)) sz) m
-  | Psall_rcl rd =>
-      Next (nextinstr_nf (rs#rd <- (Val.shl rs#rd rs#RCX)) sz) m
-  | Psalq_rcl rd =>
-      Next (nextinstr_nf (rs#rd <- (Val.shll rs#rd rs#RCX)) sz) m
-  | Psall_ri rd n =>
-      Next (nextinstr_nf (rs#rd <- (Val.shl rs#rd (Vint n))) sz) m
-  | Psalq_ri rd n =>
-      Next (nextinstr_nf (rs#rd <- (Val.shll rs#rd (Vint n))) sz) m
-  | Pshrl_rcl rd =>
-      Next (nextinstr_nf (rs#rd <- (Val.shru rs#rd rs#RCX)) sz) m
-  | Pshrq_rcl rd =>
-      Next (nextinstr_nf (rs#rd <- (Val.shrlu rs#rd rs#RCX)) sz) m
-  | Pshrl_ri rd n =>
-      Next (nextinstr_nf (rs#rd <- (Val.shru rs#rd (Vint n))) sz) m
-  | Pshrq_ri rd n =>
-      Next (nextinstr_nf (rs#rd <- (Val.shrlu rs#rd (Vint n))) sz) m
-  | Psarl_rcl rd =>
-      Next (nextinstr_nf (rs#rd <- (Val.shr rs#rd rs#RCX)) sz) m
-  | Psarq_rcl rd =>
-      Next (nextinstr_nf (rs#rd <- (Val.shrl rs#rd rs#RCX)) sz) m
-  | Psarl_ri rd n =>
-      Next (nextinstr_nf (rs#rd <- (Val.shr rs#rd (Vint n))) sz) m
-  | Psarq_ri rd n =>
-      Next (nextinstr_nf (rs#rd <- (Val.shrl rs#rd (Vint n))) sz) m
-  | Pshld_ri rd r1 n =>
-      Next (nextinstr_nf
-              (rs#rd <- (Val.or (Val.shl rs#rd (Vint n))
-                                (Val.shru rs#r1 (Vint (Int.sub Int.iwordsize n))))) sz) m
-  | Prorl_ri rd n =>
-      Next (nextinstr_nf (rs#rd <- (Val.ror rs#rd (Vint n))) sz) m
-  | Prorq_ri rd n =>
-      Next (nextinstr_nf (rs#rd <- (Val.rorl rs#rd (Vint n))) sz) m
-  | Pcmpl_rr r1 r2 =>
-      Next (nextinstr (compare_ints (rs r1) (rs r2) rs m) sz) m
-  | Pcmpq_rr r1 r2 =>
-      Next (nextinstr (compare_longs (rs r1) (rs r2) rs m) sz) m
-  | Pcmpl_ri r1 n =>
-      Next (nextinstr (compare_ints (rs r1) (Vint n) rs m) sz) m
-  | Pcmpq_ri r1 n =>
-      Next (nextinstr (compare_longs (rs r1) (Vlong n) rs m) sz) m
-  | Ptestl_rr r1 r2 =>
-      Next (nextinstr (compare_ints (Val.and (rs r1) (rs r2)) Vzero rs m) sz) m
-  | Ptestq_rr r1 r2 =>
-      Next (nextinstr (compare_longs (Val.andl (rs r1) (rs r2)) (Vlong Int64.zero) rs m) sz) m
-  | Ptestl_ri r1 n =>
-      Next (nextinstr (compare_ints (Val.and (rs r1) (Vint n)) Vzero rs m) sz) m
-  | Ptestq_ri r1 n =>
-      Next (nextinstr (compare_longs (Val.andl (rs r1) (Vlong n)) (Vlong Int64.zero) rs m) sz) m
-  | Pcmov c rd r1 =>
-      let v :=
-        match eval_testcond c rs with
-        | Some b => if b then rs#r1 else rs#rd
-        | None   => Vundef
-      end in
-      Next (nextinstr (rs#rd <- v) sz) m
-  | Psetcc c rd =>
-      Next (nextinstr (rs#rd <- (Val.of_optbool (eval_testcond c rs))) sz) m
-  (** Arithmetic operations over double-precision floats *)
-  | Paddd_ff rd r1 =>
-      Next (nextinstr (rs#rd <- (Val.addf rs#rd rs#r1)) sz) m
-  | Psubd_ff rd r1 =>
-      Next (nextinstr (rs#rd <- (Val.subf rs#rd rs#r1)) sz) m
-  | Pmuld_ff rd r1 =>
-      Next (nextinstr (rs#rd <- (Val.mulf rs#rd rs#r1)) sz) m
-  | Pdivd_ff rd r1 =>
-      Next (nextinstr (rs#rd <- (Val.divf rs#rd rs#r1)) sz) m
-  | Pnegd rd =>
-      Next (nextinstr (rs#rd <- (Val.negf rs#rd)) sz) m
-  | Pabsd rd =>
-      Next (nextinstr (rs#rd <- (Val.absf rs#rd)) sz) m
-  | Pcomisd_ff r1 r2 =>
-      Next (nextinstr (compare_floats (rs r1) (rs r2) rs) sz) m
-  | Pxorpd_f rd =>
-      Next (nextinstr_nf (rs#rd <- (Vfloat Float.zero)) sz) m
-  (** Arithmetic operations over single-precision floats *)
-  | Padds_ff rd r1 =>
-      Next (nextinstr (rs#rd <- (Val.addfs rs#rd rs#r1)) sz) m
-  | Psubs_ff rd r1 =>
-      Next (nextinstr (rs#rd <- (Val.subfs rs#rd rs#r1)) sz) m
-  | Pmuls_ff rd r1 =>
-      Next (nextinstr (rs#rd <- (Val.mulfs rs#rd rs#r1)) sz) m
-  | Pdivs_ff rd r1 =>
-      Next (nextinstr (rs#rd <- (Val.divfs rs#rd rs#r1)) sz) m
-  | Pnegs rd =>
-      Next (nextinstr (rs#rd <- (Val.negfs rs#rd)) sz) m
-  | Pabss rd =>
-      Next (nextinstr (rs#rd <- (Val.absfs rs#rd)) sz) m
-  | Pcomiss_ff r1 r2 =>
-      Next (nextinstr (compare_floats32 (rs r1) (rs r2) rs) sz) m
-  | Pxorps_f rd =>
-      Next (nextinstr_nf (rs#rd <- (Vsingle Float32.zero)) sz) m
-  (** Branches and calls *)
-  | Pjmp_l lbl =>
-      goto_label f lbl rs m
-  | Pjmp_s id sg =>
-    let addr := Genv.symbol_address ge id Ptrofs.zero in
-    match Genv.find_funct ge addr with
-    | Some _ =>
-      Next (rs#PC <- addr) m
-    | _ => Stuck
-    end
-  | Pjmp_r r sg =>
-    let addr := (rs r) in
-    match Genv.find_funct ge addr with
-    | Some _ =>
-      Next (rs#PC <- addr) m
-    | _ => Stuck
-    end
-  | Pjcc cond lbl =>
-      match eval_testcond cond rs with
-      | Some true => goto_label f lbl rs m
-      | Some false => Next (nextinstr rs sz) m
-      | None => Stuck
-      end
-  | Pjcc2 cond1 cond2 lbl =>
-      match eval_testcond cond1 rs, eval_testcond cond2 rs with
-      | Some true, Some true => goto_label f lbl rs m
-      | Some _, Some _ => Next (nextinstr rs sz) m
-      | _, _ => Stuck
-      end
-  | Pjmptbl r tbl =>
-      match rs#r with
-      | Vint n =>
-          match list_nth_z tbl (Int.unsigned n) with
-          | None => Stuck
-          | Some lbl => goto_label f lbl (rs #RAX <- Vundef #RDX <- Vundef) m
-          end
-      | _ => Stuck
-      end
-  | Pcall_s id sg =>
-    let addr := Genv.symbol_address ge id Ptrofs.zero in
-    match Genv.find_funct ge addr with
-    | Some _ =>
-      Next (rs#RA <- (Val.offset_ptr rs#PC Ptrofs.one) #PC <- addr) m
-    | _ => Stuck
-    end
-  | Pcall_r r sg =>
-    let addr := (rs r) in
-    match Genv.find_funct ge addr with
-    | Some _ =>
-      Next (rs#RA <- (Val.offset_ptr rs#PC Ptrofs.one) #PC <- addr) m
-    | _ => Stuck
-    end
-  | Pret =>
-    if check_ra_after_call ge (rs#RA) then Next (rs#PC <- (rs#RA) #RA <- Vundef) m else Stuck
-  (** Saving and restoring registers *)
-  | Pmov_rm_a rd a =>
-      exec_load (if Archi.ptr64 then Many64 else Many32) m a rs rd sz
-  | Pmov_mr_a a r1 =>
-      exec_store (if Archi.ptr64 then Many64 else Many32) m a rs r1 nil sz
-  | Pmovsd_fm_a rd a =>
-      exec_load Many64 m a rs rd sz
-  | Pmovsd_mf_a a r1 =>
-      exec_store Many64 m a rs r1 nil sz
-  (** Pseudo-instructions *)
-  | Plabel lbl =>
-      Next (nextinstr rs sz) m
-  | Pallocframe fsz ofs_ra ofs_link =>
-    if zle 0 fsz then
-    match rs # PC with
-    |Vptr (Global id) _
-     =>
-     let (m0,path) := Mem.alloc_frame m id in
-     let (m1, stk) := Mem.alloc m0 0 fsz in
-     match Mem.record_frame (Mem.push_stage m1) (Memory.mk_frame fsz) with
-     |None => Stuck
-     |Some m2 =>
-      let sp := Vptr stk Ptrofs.zero in
-      match Mem.storev Mptr m2 (Val.offset_ptr sp ofs_ra) rs#RA with
-      | None => Stuck
-      | Some m3 =>
-        match Mem.storev Mptr m3 (Val.offset_ptr sp ofs_link) rs#RSP with
-        | None => Stuck
-        | Some m4 => Next (nextinstr (rs #RAX <- (rs#RSP) #RSP <- sp) sz) m4
-        end
-      end
-     end
-    |_ => Stuck
-    end else Stuck
-  | Pfreeframe fsz ofs_ra ofs_link =>
-    if zle 0 fsz then
-      match loadvv Mptr m (Val.offset_ptr rs#RSP ofs_ra) with
-      | None => Stuck
-      | Some ra =>
-          match Mem.loadv Mptr m (Val.offset_ptr rs#RSP ofs_link) with
-          | None => Stuck
-          | Some sp =>
-              match rs#RSP with
-              | Vptr stk ofs =>
-                  if check_topframe fsz (Mem.astack (Mem.support m)) then
-                  if Val.eq sp (parent_sp_stree (Mem.stack (Mem.support m))) then
-                  if Val.eq (Vptr stk ofs) (top_sp_stree (Mem.stack (Mem.support m))) then
-                  match Mem.free m stk 0 fsz with
-                  | None => Stuck
-                  | Some m' =>
-                    match Mem.return_frame m' with
-                    | None => Stuck
-                    | Some m'' =>
-                      match Mem.pop_stage m'' with
-                        | None => Stuck
-                        | Some m''' =>
-                        Next (nextinstr (rs#RSP <- sp #RA <- ra) sz) m'''
-                      end
-                    end
-                  end else Stuck else Stuck else Stuck
-              | _ => Stuck
-              end
-          end
-      end else Stuck
-  | Pbuiltin ef args res =>
-      Stuck                             (**r treated specially below *)
-  (** The following instructions and directives are not generated
-      directly by [Asmgen], so we do not model them. *)
-  | Padcl_ri _ _
-  | Padcl_rr _ _
-  | Paddl_mi _ _
-  | Paddl_rr _ _
-  | Pbsfl _ _
-  | Pbsfq _ _
-  | Pbsrl _ _
-  | Pbsrq _ _
-  | Pbswap64 _
-  | Pbswap32 _
-  | Pbswap16 _
-  | Pcfi_adjust _
-  | Pfmadd132 _ _ _
-  | Pfmadd213 _ _ _
-  | Pfmadd231 _ _ _
-  | Pfmsub132 _ _ _
-  | Pfmsub213 _ _ _
-  | Pfmsub231 _ _ _
-  | Pfnmadd132 _ _ _
-  | Pfnmadd213 _ _ _
-  | Pfnmadd231 _ _ _
-  | Pfnmsub132 _ _ _
-  | Pfnmsub213 _ _ _
-  | Pfnmsub231 _ _ _
-  | Pmaxsd _ _
-  | Pminsd _ _
-  | Pmovb_rm _ _
-  | Pmovq_rf _ _
-  | Pmovsq_rm _ _
-  | Pmovsq_mr _ _
-  | Pmovsb
-  | Pmovsw
-  | Pmovw_rm _ _
-  | Pnop
-  | Prep_movsl
-  | Psbbl_rr _ _
-  | Psqrtsd _ _
-  | Psubl_ri _ _
-  | Psubq_ri _ _ => Stuck
-  end.
-
-(* maybe useful to prove SSAsm -> RealAsm_1 *)
   Definition exec_instr f i rs (m: mem) :=
     let isz := Ptrofs.repr (instr_size i) in
     match i with
@@ -545,11 +33,11 @@ Definition exec_instr_asm (f: function) (i: instruction) (rs: regset) (m: mem) :
       match Mem.storev Mptr m (Val.offset_ptr sp ofs_link) psp with
         |None => Stuck
         |Some m1 =>
-      Next (nextinstr (rs #RAX <- (Val.offset_ptr (rs RSP) (Ptrofs.repr (size_chunk Mptr))) #RSP <- sp) isz) m1
+      Next (nextinstr isz (rs #RAX <- (Val.offset_ptr (rs RSP) (Ptrofs.repr (size_chunk Mptr))) #RSP <- sp)) m1
       end
     | Pfreeframe sz ofs_ra ofs_link =>
       let sp := Val.offset_ptr (rs RSP) (Ptrofs.sub (Ptrofs.repr (align sz 8)) (Ptrofs.repr (size_chunk Mptr))) in
-      Next (nextinstr (rs#RSP <- sp) isz) m
+      Next (nextinstr isz (rs#RSP <- sp)) m
     | Pcall_s i sg =>
       let sp := Val.offset_ptr (rs RSP) (Ptrofs.neg (Ptrofs.repr (size_chunk Mptr))) in
       match Mem.storev Mptr m sp (Val.offset_ptr rs#PC isz) with
@@ -577,7 +65,7 @@ Definition exec_instr_asm (f: function) (i: instruction) (rs: regset) (m: mem) :
                  #PC <- ra
                  #RA <- Vundef) m
       end
-    | _ => exec_instr_asm f i rs m
+    | _ => exec_instr instr_size ge f i rs m
     end.
 
   Inductive step  : state -> trace -> state -> Prop :=
@@ -585,20 +73,19 @@ Definition exec_instr_asm (f: function) (i: instruction) (rs: regset) (m: mem) :
       forall b ofs f i rs m rs' m',
         rs PC = Vptr b ofs ->
         Genv.find_funct_ptr ge b = Some (Internal f) ->
-        find_instr (Ptrofs.unsigned ofs) (fn_code f) = Some i ->
+        find_instr instr_size (Ptrofs.unsigned ofs) (fn_code f) = Some i ->
         exec_instr f i rs m = Next rs' m' ->
         step (State rs m) E0 (State rs' m')
   | exec_step_builtin:
       forall b ofs f ef args res rs m vargs t vres rs' m',
         rs PC = Vptr b ofs ->
         Genv.find_funct_ptr ge b = Some (Internal f) ->
-        find_instr (Ptrofs.unsigned ofs) f.(fn_code) = Some (Pbuiltin ef args res) ->
+        find_instr instr_size (Ptrofs.unsigned ofs) f.(fn_code) = Some (Pbuiltin ef args res) ->
         eval_builtin_args ge rs (rs RSP) m args vargs ->
         external_call ef ge vargs m t vres m' ->
-        rs' = nextinstr_nf
+        rs' = nextinstr_nf (Ptrofs.repr (instr_size (Pbuiltin ef args res)))
                 (set_res res vres
-                         (undef_regs (map preg_of (destroyed_by_builtin ef)) rs))
-                         (Ptrofs.repr (instr_size (Pbuiltin ef args res))) ->
+                         (undef_regs (map preg_of (destroyed_by_builtin ef)) rs)) ->
         step (State rs m) t (State rs' m')
   | exec_step_external:
       forall b ef args res rs m t rs' m',
@@ -734,8 +221,8 @@ Section WITHGETGE.
     Qed. *)
 
     Lemma goto_label_eq : forall (i:instruction) f f' l rs m,
-        (forall lbl ofs, label_pos lbl ofs (fn_code f) = label_pos lbl ofs (fn_code f')) ->
-        goto_label ge f l rs m = goto_label tge f' l rs m.
+        (forall lbl ofs, label_pos instr_size lbl ofs (fn_code f) = label_pos instr_size lbl ofs (fn_code f')) ->
+        goto_label instr_size ge f l rs m = goto_label instr_size tge f' l rs m.
     Proof.
       intros.
       unfold goto_label. destr.
@@ -749,7 +236,7 @@ Section WITHGETGE.
     Qed.
 
     Lemma exec_instr_same : forall (i:instruction) f f' i rs m,
-        (forall lbl ofs, label_pos lbl ofs (fn_code f) = label_pos lbl ofs (fn_code f')) ->
+        (forall lbl ofs, label_pos instr_size lbl ofs (fn_code f) = label_pos instr_size lbl ofs (fn_code f')) ->
         exec_instr ge f i rs m = exec_instr tge f' i rs m.
     Proof.
       intros i f f' i0 rs m LP.
@@ -870,63 +357,63 @@ Section WFASM.
 
       wf_asm_alloc_only_at_beginning:
         forall o sz ora olink,
-          find_instr o (fn_code f) = Some (Pallocframe sz ora olink) ->
+          find_instr instr_size o (fn_code f) = Some (Pallocframe sz ora olink) ->
           o = 0;
 
       wf_asm_alloc_at_beginning:
-        find_instr 0 (fn_code f) = Some (make_palloc f);
+        find_instr instr_size 0 (fn_code f) = Some (make_palloc f);
 
       wf_asm_after_freeframe:
         forall i o,
-          find_instr (Ptrofs.unsigned o) (fn_code f) = Some i ->
+          find_instr instr_size (Ptrofs.unsigned o) (fn_code f) = Some i ->
           is_free i ->
           exists i' ,
-            find_instr (Ptrofs.unsigned (Ptrofs.add o (Ptrofs.repr (instr_size i)))) (fn_code f) = Some i' /\
+            find_instr instr_size (Ptrofs.unsigned (Ptrofs.add o (Ptrofs.repr (instr_size i)))) (fn_code f) = Some i' /\
             (i' = Pret \/ is_jmp i' );
 
       wf_asm_ret_jmp_comes_after_freeframe:
         forall i o,
-          find_instr (Ptrofs.unsigned o) (fn_code f) = Some i ->
+          find_instr instr_size (Ptrofs.unsigned o) (fn_code f) = Some i ->
           i = Pret \/ is_jmp i ->
           exists o' ifree,
-            find_instr (Ptrofs.unsigned o') (fn_code f) = Some ifree /\
+            find_instr instr_size (Ptrofs.unsigned o') (fn_code f) = Some ifree /\
             is_free ifree /\
             Ptrofs.unsigned o' + instr_size ifree = Ptrofs.unsigned o;
 
       wf_asm_code_bounded:
-        0 <= code_size (fn_code f) <= Ptrofs.max_unsigned;
+        0 <= code_size instr_size (fn_code f) <= Ptrofs.max_unsigned;
 
       wf_asm_builtin_not_PC:
         forall o ef args res,
-          find_instr o (fn_code f) = Some (Pbuiltin ef args res) ->
+          find_instr instr_size o (fn_code f) = Some (Pbuiltin ef args res) ->
           ~ in_builtin_res res PC /\
           ~ in_builtin_res res RSP
           /\ Forall (fun arg : builtin_arg preg => ~ in_builtin_arg arg RA) args;
 
       wf_asm_jmp_no_rsp:
         forall o (r: ireg) sg,
-          find_instr o (fn_code f) = Some (Pjmp_r r sg) ->
+          find_instr instr_size o (fn_code f) = Some (Pjmp_r r sg) ->
           r <> RSP;
 
       wf_asm_call_no_rsp:
         forall o (r: ireg) sg,
-          find_instr o (fn_code f) = Some (Pcall_r r sg) ->
+          find_instr instr_size o (fn_code f) = Some (Pcall_r r sg) ->
           r <> RSP;
 
       wf_asm_free_spec:
         forall o sz ora olink,
-          find_instr o (fn_code f) = Some (Pfreeframe sz ora olink) ->
+          find_instr instr_size o (fn_code f) = Some (Pfreeframe sz ora olink) ->
           sz = fn_stacksize f /\ ora = Ptrofs.sub (Ptrofs.repr (align sz 8)) (Ptrofs.repr (size_chunk Mptr));
 
       wf_allocframe_repr:
         forall o sz ora olink,
-          find_instr o (fn_code f) = Some (Pallocframe sz ora olink) ->
+          find_instr instr_size o (fn_code f) = Some (Pallocframe sz ora olink) ->
           align sz 8 - size_chunk Mptr =
           Ptrofs.unsigned (Ptrofs.sub (Ptrofs.repr (align sz 8)) (Ptrofs.repr (size_chunk Mptr)));
 
       wf_freeframe_repr:
         forall o sz ora olink,
-          find_instr o (fn_code f) = Some (Pfreeframe sz ora olink) ->
+          find_instr instr_size o (fn_code f) = Some (Pfreeframe sz ora olink) ->
           Ptrofs.repr (align sz 8 - size_chunk Mptr) = Ptrofs.sub (Ptrofs.repr (align sz 8)) (Ptrofs.repr (size_chunk Mptr));
     }.
 
@@ -1027,31 +514,30 @@ Section WFASM.
     apply not_in_builtin_arg_dec.
   Defined.
 
-  Hypothesis instr_size_repr : forall i, 0 <= instr_size i <= Ptrofs.max_unsigned.
-  Hypothesis instr_size_positive : forall i, 0 < instr_size i.
+  Hypothesis instr_size_bound : forall i, 0 < instr_size i <= Ptrofs.max_unsigned.
 
-  Lemma code_size_non_neg: forall c, 0 <= code_size c.
+  Lemma code_size_non_neg: forall c, 0 <= code_size instr_size c.
   Proof.
-    intros. induction c; simpl. lia. generalize (instr_size_positive a); lia.
+    intros. induction c; simpl. lia. generalize (instr_size_bound a); lia.
   Qed.
 
   Lemma find_instr_bound:
     forall c o i,
-      find_instr o c = Some i ->
-      o + instr_size i <= code_size c.
+      find_instr instr_size o c = Some i ->
+      o + instr_size i <= code_size instr_size c.
   Proof.
     induction c; simpl; intros; eauto. congruence.
-    destr_in H. inv H. generalize (code_size_non_neg c) (instr_size_positive i). lia.
+    destr_in H. inv H. generalize (code_size_non_neg c) (instr_size_bound i). lia.
     apply IHc in H. lia.
   Qed.
 
   Lemma find_instr_pos_positive:
         forall c o i,
-          find_instr o c = Some i ->
+          find_instr instr_size o c = Some i ->
           0 <= o.
    Proof.
      induction c; intros; simpl; inv H. destr_in H1. lia.
-     eapply IHc in H1. generalize (instr_size_positive a). lia.
+     eapply IHc in H1. generalize (instr_size_bound a). lia.
    Qed.
 (*
   Lemma instr_size_repr : 0 <= 1 <= Ptrofs.max_unsigned.
@@ -1061,16 +547,16 @@ Section WFASM.
 
   Lemma code_bounded_repr':
     forall c
-      (RNG: 0 <= code_size c <= Ptrofs.max_unsigned)
+      (RNG: 0 <= code_size instr_size c <= Ptrofs.max_unsigned)
       i o
-      (FI: find_instr o c = Some i)
+      (FI: find_instr instr_size o c = Some i)
       sz
       (LE: 0 <= sz <= instr_size i),
       Ptrofs.unsigned (Ptrofs.add (Ptrofs.repr o) (Ptrofs.repr sz)) = o + sz.
   Proof.
     intros.
     unfold Ptrofs.add.
-    rewrite (Ptrofs.unsigned_repr sz). 2: generalize (instr_size_repr i); lia.
+    rewrite (Ptrofs.unsigned_repr sz). 2: generalize (instr_size_bound i); lia.
     generalize (find_instr_bound _ _ _ FI) (find_instr_pos_positive _ _ _ FI). intros.
     rewrite (Ptrofs.unsigned_repr o) by lia.
     apply Ptrofs.unsigned_repr; lia.
@@ -1078,9 +564,9 @@ Section WFASM.
 
   Lemma code_bounded_repr:
     forall c
-      (RNG: 0 <= code_size c <= Ptrofs.max_unsigned)
+      (RNG: 0 <= code_size instr_size c <= Ptrofs.max_unsigned)
       i o
-      (FI: find_instr (Ptrofs.unsigned o) c = Some i)
+      (FI: find_instr instr_size (Ptrofs.unsigned o) c = Some i)
       sz
       (LE: 0 <= sz <= instr_size i),
       Ptrofs.unsigned (Ptrofs.add o (Ptrofs.repr sz)) = Ptrofs.unsigned o + sz.
@@ -1094,7 +580,7 @@ Section WFASM.
   Lemma wf_asm_pc_repr' : forall f : function,
        wf_asm_function f ->
        forall (i : instruction) (o : ptrofs),
-       find_instr (Ptrofs.unsigned o) (fn_code f) = Some i ->
+       find_instr instr_size (Ptrofs.unsigned o) (fn_code f) = Some i ->
        forall sz : Z, 0 <= sz <= instr_size i ->
        Ptrofs.unsigned (Ptrofs.add o (Ptrofs.repr sz)) = Ptrofs.unsigned o + sz.
   Proof.
@@ -1125,7 +611,7 @@ Section WFASM.
     match fn_code f with
     | nil => false
     | a::r => is_make_palloc_dec a f && check_asm_body f false r
-    end && zle (code_size (fn_code f)) Ptrofs.max_unsigned.
+    end && zle (code_size instr_size (fn_code f)) Ptrofs.max_unsigned.
 
   Lemma check_asm_body_no_alloc:
     forall f c b i,
@@ -1148,19 +634,19 @@ Section WFASM.
   Lemma find_instr_app:
     forall a o b,
       0 <= o ->
-      find_instr (o + code_size a) (a ++ b) = find_instr o b.
+      find_instr instr_size (o + code_size instr_size a) (a ++ b) = find_instr instr_size o b.
   Proof.
     induction a; simpl; intros; eauto.
     f_equal. lia.
     rewrite pred_dec_false.
     rewrite <- (IHa o b). f_equal. lia. lia.
-    generalize (code_size_non_neg a0). generalize (instr_size_positive a). lia.
+    generalize (code_size_non_neg a0). generalize (instr_size_bound a). lia.
   Qed.
 
   Lemma find_instr_app':
     forall a o b,
-      code_size a <= o ->
-      find_instr o (a ++ b) = find_instr (o - code_size a) b.
+      code_size instr_size a <= o ->
+      find_instr instr_size o (a ++ b) = find_instr instr_size (o - code_size instr_size a) b.
   Proof.
     intros.
     rewrite <- (find_instr_app a _ b). f_equal. lia. lia.
@@ -1168,19 +654,19 @@ Section WFASM.
 
   Lemma find_instr_split:
     forall c o i,
-      find_instr o c = Some i ->
-      exists a b, c = a ++ i :: b /\ o = code_size a.
+      find_instr instr_size o c = Some i ->
+      exists a b, c = a ++ i :: b /\ o = code_size instr_size a.
   Proof.
     induction c; simpl; intros; eauto. congruence.
     destr_in H. inv H. eexists nil, c; simpl. split; auto.
     edestruct IHc as (aa & b & EQ & SZ). apply H. subst.
     exists (a::aa), b; simpl; split; auto.
-    generalize (instr_size_positive a). lia.
+    generalize (instr_size_bound a). lia.
   Qed.
 
   Lemma find_instr_app_pres: forall f1 f2 ofs i,
-      find_instr ofs f1 = Some i ->
-      find_instr ofs (f1 ++ f2) = Some i.
+      find_instr instr_size ofs f1 = Some i ->
+      find_instr instr_size ofs (f1 ++ f2) = Some i.
   Proof.
     induction f1 as [|i1 f1].
     - cbn. intros; congruence.
@@ -1190,7 +676,7 @@ Section WFASM.
 
   Lemma code_size_app:
     forall c1 c2,
-      code_size (c1 ++ c2) = code_size c1 + code_size c2.
+      code_size instr_size (c1 ++ c2) = code_size instr_size c1 + code_size instr_size c2.
   Proof.
     induction c1; simpl; intros; eauto. rewrite IHc1. lia.
   Qed.
@@ -1302,7 +788,7 @@ Section WFASM.
 
   Lemma find_instr_in:
     forall c pos i,
-      find_instr pos c = Some i -> In i c.
+      find_instr instr_size pos c = Some i -> In i c.
   Proof.
     induction c; simpl. intros; discriminate.
     intros until i. case (zeq pos 0); intros.
@@ -1339,55 +825,60 @@ Section WFASM.
       apply andb_true_iff in B. destruct B as (B & CHK).
       unfold check_ret_or_jmp in CHK. apply andb_true_iff in CHK. destruct CHK as (CHK & _). destr_in CHK; try (right; constructor).
       unfold Ptrofs.add.
-      rewrite (Ptrofs.unsigned_repr (code_size a)).
-      rewrite (Ptrofs.unsigned_repr _ (instr_size_repr i)).
+      rewrite (Ptrofs.unsigned_repr (code_size instr_size a)).
+      rewrite (Ptrofs.unsigned_repr (instr_size i) ).
       rewrite Ptrofs.unsigned_repr. lia.
       simpl in SIZE. rewrite code_size_app in SIZE. simpl in SIZE.
-      generalize (code_size_non_neg a) (instr_size_positive i) (instr_size_positive i0) (code_size_non_neg b)
-                 (instr_size_positive (make_palloc f)). lia.
+      generalize (code_size_non_neg a) (instr_size_bound i) (instr_size_bound i0) (code_size_non_neg b)
+                 (instr_size_bound (make_palloc f)); lia.
+      generalize (instr_size_bound i). lia.
       simpl in SIZE. rewrite code_size_app in SIZE. simpl in SIZE.
-      generalize (code_size_non_neg a) (instr_size_positive i) (instr_size_positive i0) (code_size_non_neg b)
-                 (instr_size_positive (make_palloc f)). lia.
+      generalize (code_size_non_neg a) (instr_size_bound i) (instr_size_bound i0) (code_size_non_neg b)
+                 (instr_size_bound (make_palloc f)). simpl in SIZE. lia.
       unfold Ptrofs.add.
-      rewrite (Ptrofs.unsigned_repr (code_size a)).
-      rewrite (Ptrofs.unsigned_repr _ (instr_size_repr i)).
-      rewrite Ptrofs.unsigned_repr. generalize (instr_size_positive i); lia.
+      rewrite (Ptrofs.unsigned_repr (code_size instr_size a)).
+      rewrite (Ptrofs.unsigned_repr (instr_size i)).
+      rewrite Ptrofs.unsigned_repr. generalize (instr_size_bound i); lia.
       simpl in SIZE. rewrite code_size_app in SIZE. simpl in SIZE.
-      generalize (code_size_non_neg a) (instr_size_positive i) (code_size_non_neg b)
-                 (instr_size_positive (make_palloc f)). lia.
+      generalize (code_size_non_neg a) (instr_size_bound i) (code_size_non_neg b)
+                 (instr_size_bound (make_palloc f)). lia.
+      generalize (instr_size_bound i). lia.
       simpl in SIZE. rewrite code_size_app in SIZE. simpl in SIZE.
-      generalize (code_size_non_neg a) (instr_size_positive i) (code_size_non_neg b)
-                 (instr_size_positive (make_palloc f)). lia.
+      generalize (code_size_non_neg a) (instr_size_bound i) (code_size_non_neg b)
+                 (instr_size_bound (make_palloc f)). lia.
       unfold Ptrofs.add.
-      rewrite (Ptrofs.unsigned_repr (code_size a)).
-      rewrite (Ptrofs.unsigned_repr _ (instr_size_repr i)).
-      rewrite Ptrofs.unsigned_repr. generalize (instr_size_positive i); lia.
+      rewrite (Ptrofs.unsigned_repr (code_size instr_size a)).
+      rewrite (Ptrofs.unsigned_repr (instr_size i)).
+      rewrite Ptrofs.unsigned_repr. generalize (instr_size_bound i); lia.
       simpl in SIZE. rewrite code_size_app in SIZE. simpl in SIZE.
-      generalize (code_size_non_neg a) (instr_size_positive i) (code_size_non_neg b)
-                 (instr_size_positive (make_palloc f)). lia.
+      generalize (code_size_non_neg a) (instr_size_bound i) (code_size_non_neg b)
+                 (instr_size_bound (make_palloc f)). lia.
+      generalize (instr_size_bound i). lia.
       simpl in SIZE. rewrite code_size_app in SIZE. simpl in SIZE.
-      generalize (code_size_non_neg a) (instr_size_positive i) (code_size_non_neg b)
-                 (instr_size_positive (make_palloc f)). lia.
+      generalize (code_size_non_neg a) (instr_size_bound i) (code_size_non_neg b)
+                 (instr_size_bound (make_palloc f)). lia.
       unfold Ptrofs.add.
-      rewrite (Ptrofs.unsigned_repr _ (instr_size_repr i)).
+      rewrite (Ptrofs.unsigned_repr (instr_size i)).
       rewrite (Ptrofs.unsigned_repr (Ptrofs.unsigned o - _)).
       rewrite ! Ptrofs.unsigned_repr. lia.
       generalize (find_instr_bound _ _ _ H) (find_instr_pos_positive _ _ _ H).
-      generalize (instr_size_positive i)
-                 (instr_size_positive (make_palloc f)). lia.
+      generalize (instr_size_bound i)
+                 (instr_size_bound (make_palloc f)). lia.
       generalize (find_instr_bound _ _ _ H) (find_instr_pos_positive _ _ _ H).
-      generalize (instr_size_positive i)
-                 (instr_size_positive (make_palloc f)). lia.
+      generalize (instr_size_bound i)
+                 (instr_size_bound (make_palloc f)). lia.
       generalize (find_instr_bound _ _ _ H) (find_instr_pos_positive _ _ _ H).
-      generalize (instr_size_positive i)
-                 (instr_size_positive (make_palloc f)). lia.
+      generalize (instr_size_bound i)
+                 (instr_size_bound (make_palloc f)). lia.
+      generalize (instr_size_bound i). lia.
       unfold Ptrofs.add.
-      rewrite (Ptrofs.unsigned_repr _ (instr_size_repr i)).
+      rewrite (Ptrofs.unsigned_repr (instr_size i)).
       rewrite Ptrofs.unsigned_repr.
-      generalize (Ptrofs.unsigned_range o) (instr_size_positive i); lia.
+      generalize (Ptrofs.unsigned_range o) (instr_size_bound i); lia.
       generalize (find_instr_bound _ _ _ H) (find_instr_pos_positive _ _ _ H).
-      generalize (instr_size_positive i)
-                 (instr_size_positive (make_palloc f)). lia.
+      generalize (instr_size_bound i)
+                 (instr_size_bound (make_palloc f)). lia.
+      generalize (instr_size_bound i). lia.
     - destruct i0 as (i0 & _). subst. rewrite CODE. simpl.
       intros i o FI ROJ.
       destr_in FI. inv FI. destruct ROJ as [ROJ|ROJ]; inv ROJ.
@@ -1397,36 +888,39 @@ Section WFASM.
       exists (Ptrofs.sub o (Ptrofs.repr (instr_size i0))), i0.
       rewrite pred_dec_false.
       replace (Ptrofs.unsigned (Ptrofs.sub o (Ptrofs.repr (instr_size i0))) - instr_size (make_palloc f)) 
-        with (0 + code_size a0). rewrite app_ass.
+        with (0 + code_size instr_size a0). rewrite app_ass.
       rewrite find_instr_app. simpl. split; auto. split. auto.
-      unfold Ptrofs.sub. 
-      rewrite (Ptrofs.unsigned_repr _ (instr_size_repr i0)).
+      unfold Ptrofs.sub.
+      rewrite (Ptrofs.unsigned_repr (instr_size i0)).
       rewrite Ptrofs.unsigned_repr. lia.
       generalize (find_instr_bound _ _ _ FI) (find_instr_pos_positive _ _ _ FI). intros.
       simpl in *. rewrite ! code_size_app in *. simpl in *.
-      generalize (code_size_non_neg a0) (instr_size_positive i) (instr_size_positive i0) (code_size_non_neg b)
-                 (instr_size_positive (make_palloc f)). lia.
+      generalize (code_size_non_neg a0) (instr_size_bound i) (instr_size_bound i0) (code_size_non_neg b)
+                 (instr_size_bound (make_palloc f)). lia.
+      generalize (instr_size_bound i0). lia.
       lia.
       unfold Ptrofs.sub. 
-      rewrite (Ptrofs.unsigned_repr _ (instr_size_repr i0)).
+      rewrite (Ptrofs.unsigned_repr (instr_size i0)).
       rewrite Ptrofs.unsigned_repr.
       simpl in *. rewrite ! code_size_app in *. simpl in *. lia.
       generalize (find_instr_bound _ _ _ FI) (find_instr_pos_positive _ _ _ FI). intros.
       simpl in *. rewrite ! code_size_app in *. simpl in *.
-      generalize (code_size_non_neg a0) (instr_size_positive i) (instr_size_positive i0) (code_size_non_neg b)
-                 (instr_size_positive (make_palloc f)). lia.
+      generalize (code_size_non_neg a0) (instr_size_bound i) (instr_size_bound i0) (code_size_non_neg b)
+                 (instr_size_bound (make_palloc f)). lia.
+      generalize (instr_size_bound i0). lia.
       unfold Ptrofs.sub. 
-      rewrite (Ptrofs.unsigned_repr _ (instr_size_repr i0)).
+      rewrite (Ptrofs.unsigned_repr (instr_size i0)).
       rewrite Ptrofs.unsigned_repr.
       simpl in *. rewrite ! code_size_app in *. simpl in *.
       generalize (find_instr_bound _ _ _ FI) (find_instr_pos_positive _ _ _ FI). intros. 
       simpl in *. rewrite ! code_size_app in *. simpl in *.
-      generalize (code_size_non_neg a0) (instr_size_positive i) (instr_size_positive i0) (code_size_non_neg b)
-                 (instr_size_positive (make_palloc f)). lia.
+      generalize (code_size_non_neg a0) (instr_size_bound i) (instr_size_bound i0) (code_size_non_neg b)
+                 (instr_size_bound (make_palloc f)). lia.
       generalize (find_instr_bound _ _ _ FI) (find_instr_pos_positive _ _ _ FI). intros. 
       simpl in *. rewrite ! code_size_app in *. simpl in *.
-      generalize (code_size_non_neg a0) (instr_size_positive i) (instr_size_positive i0) (code_size_non_neg b)
-                 (instr_size_positive (make_palloc f)). lia.
+      generalize (code_size_non_neg a0) (instr_size_bound i) (instr_size_bound i0) (code_size_non_neg b)
+                 (instr_size_bound (make_palloc f)). lia.
+      generalize (instr_size_bound i0). lia.
     - rewrite CODE; split; auto.
       generalize (code_size_non_neg (i::c)). lia.
     - destruct i0 as (i0 & _). subst. rewrite CODE. simpl.
@@ -1463,15 +957,15 @@ Section WFASM.
 
   Lemma wf_asm_pc_repr:
     forall f (WF: wf_asm_function f) i o,
-      find_instr (Ptrofs.unsigned o) (fn_code f) = Some i ->
+      find_instr instr_size (Ptrofs.unsigned o) (fn_code f) = Some i ->
       Ptrofs.unsigned (Ptrofs.add o (Ptrofs.repr (instr_size i))) = Ptrofs.unsigned o + instr_size i.
   Proof.
-    intros; eapply wf_asm_pc_repr'; eauto. generalize (instr_size_positive i); lia.
+    intros; eapply wf_asm_pc_repr'; eauto. generalize (instr_size_bound i); lia.
   Qed.
 
   Lemma wf_asm_wf_allocframe:
     forall f (WF: wf_asm_function f) o sz ora olink
-      (FI: find_instr o (fn_code f) = Some (Pallocframe sz ora olink)),
+      (FI: find_instr instr_size o (fn_code f) = Some (Pallocframe sz ora olink)),
       make_palloc f = Pallocframe sz ora olink.
   Proof.
     intros.
@@ -1480,12 +974,6 @@ Section WFASM.
   Qed.
 
 End WFASM.
-
-End INSTRSIZE.
-(* RealAsm senmantic version 1: instr_size == 1*)
-
-Definition instr_size_1 : instruction -> Z := fun i => 1.
-
 
 Definition rs_state s :=
   let '(State rs _) := s in rs.
@@ -1566,16 +1054,16 @@ Qed.
     Lemma exec_instr_invar_same:
       forall f i rs1 m1,
         stk_unrelated_instr i = true ->
-        exec_instr instr_size_1 ge f i rs1 m1 = SSAsm.exec_instr ge f i rs1 m1.
+        exec_instr ge f i rs1 m1 = SSAsm.exec_instr instr_size ge f i rs1 m1.
     Proof.
       intros f i rs1 m1 SI.
-      destruct i; simpl in SI; simpl; unfold instr_size_1; simpl; try reflexivity; congruence.
+      destruct i; simpl in SI;  simpl; try reflexivity; congruence.
     Qed.
 
     Lemma exec_instr_invar_same':
       forall f i rs1 m1,
         stk_unrelated_instr i = true ->
-        Asm.exec_instr ge f i rs1 m1 = SSAsm.exec_instr ge f i rs1 m1.
+        Asm.exec_instr instr_size ge f i rs1 m1 = SSAsm.exec_instr instr_size ge f i rs1 m1.
     Proof.
       intros f i rs1 m1 SI.
       destruct i; simpl in SI; simpl; try congruence.
@@ -1583,9 +1071,9 @@ Qed.
 
     Lemma exec_instr_invar_inv:
       forall f i rs1 m1 rs2 m2,
-        asm_instr_unchange_rsp i ->
+        asm_instr_unchange_rsp instr_size i ->
         stk_unrelated_instr i = true ->
-        exec_instr (instr_size_1) ge f i rs1 m1 = Next rs2 m2 ->
+        exec_instr ge f i rs1 m1 = Next rs2 m2 ->
         real_asm_inv (State rs1 m1) ->
         real_asm_inv (State rs2 m2).
     Proof.
@@ -1593,7 +1081,7 @@ Qed.
       erewrite exec_instr_invar_same in EI; eauto.
       erewrite <- exec_instr_invar_same' in EI; eauto.
       exploit NORSP; eauto. intro EQ.
-      generalize (asm_prog_unchange_sup i INVAR _ _ _ _ _ _ EI). intros (A & B).
+      generalize (asm_prog_unchange_sup instr_size i INVAR _ _ _ _ _ _ EI). intros (A & B).
       constructor.
       + red in RSPPTR; red. simpl in *; rewrite <- EQ. eauto.
       + red in BSTACKPERM; red. simpl in *. setoid_rewrite <- B. eauto.
@@ -1643,12 +1131,12 @@ Qed.
     Definition asm_prog_no_rsp (ge: Genv.t Asm.fundef unit):=
       forall b f,
         Genv.find_funct_ptr ge b = Some (Internal f) ->
-        asm_code_no_rsp (fn_code f).
+        asm_code_no_rsp instr_size (fn_code f).
 
   Definition wf_asm_prog (ge: Genv.t Asm.fundef unit):=
       forall b f,
         Genv.find_funct_ptr ge b = Some (Internal f) ->
-        wf_asm_function instr_size_1 f.
+        wf_asm_function f.
 
 (*Lemma nextinstr_nf_pc: forall rs sz, nextinstr_nf rs sz PC = Val.offset_ptr (rs PC) sz.
 Proof.
@@ -1657,16 +1145,16 @@ Proof.
 Qed. *)
 
 Lemma nextinstr_rsp:
-  forall rs sz,
-    nextinstr rs sz RSP= rs RSP.
+  forall sz rs,
+    nextinstr sz rs RSP= rs RSP.
 Proof.
   unfold nextinstr.
   intros; rewrite Pregmap.gso; congruence.
 Qed.
 
 Lemma nextinstr_nf_rsp:
-  forall rs sz,
-    nextinstr_nf rs sz RSP = rs RSP.
+  forall sz rs,
+    nextinstr_nf sz rs RSP = rs RSP.
 Proof.
   unfold nextinstr_nf.
   intros. rewrite nextinstr_rsp.
@@ -1676,7 +1164,7 @@ Qed.
 
     Lemma real_asm_inv_inv:
       forall (prog_no_rsp: asm_prog_no_rsp ge) (WF: wf_asm_prog ge) s1 t s2,
-        (step instr_size_1) ge s1 t s2 ->
+        step ge s1 t s2 ->
         real_asm_inv s1 ->
         real_asm_inv s2.
     Proof.
@@ -1785,4 +1273,4 @@ Qed.
     Qed.
 
 End INVARIANT.
-
+End INSTRSIZE.
