x86/RealAsmgen.v
@@ -7,8 +7,11 @@ Require Import Op Locations Mach Asm RealAsm.
 Local Open Scope string_scope.
 Local Open Scope error_monad_scope.
 
+Section INSTRSIZE.
+Variable instr_size : instruction -> Z.
+
 Definition transf_function (f: Asm.function) : res Asm.function :=
-  if wf_asm_function_check instr_size_1 f then
+  if wf_asm_function_check instr_size f then
     OK f
   else
     Error (msg "asm_function_is_not_wellformed").
@@ -18,3 +21,5 @@ Definition transf_fundef (f: Asm.fundef) : res Asm.fundef :=
 
 Definition transf_program (p: Asm.program) : res Asm.program :=
   transform_partial_program transf_fundef p.
+
+End INSTRSIZE.
