x86/RealAsmproof.v
@@ -15,13 +15,15 @@ Require Import Values.
 Require Import Conventions1.
 Require Import AsmFacts.
 Require Import SSAsm RealAsm RealAsmgen.
-Require Import AsmRegs RealAsmRegs.
+Require Import AsmRegs.
 Require Import Errors.
 Require Import Linking.
 
   Section PRESERVATION.
-
+ 
   Variable prog: Asm.program.
+  Variable instr_size: instruction -> Z.
+  Hypothesis instr_size_bound : forall i, 0 < instr_size i <= Ptrofs.max_unsigned.
   Let ge := Genv.globalenv prog.
 
   Definition pc_at (s: state): option ((function * instruction) + external_function) :=
@@ -30,7 +32,7 @@ Require Import Linking.
     | Vptr b o =>
       match Genv.find_funct_ptr ge b with
       | Some (Internal f) =>
-        match find_instr instr_size_1 (Ptrofs.unsigned o) (fn_code f) with
+        match find_instr instr_size (Ptrofs.unsigned o) (fn_code f) with
         | Some i => Some (inl (f,i))
         | None => None
         end
@@ -102,7 +104,7 @@ Require Import Linking.
     vm_compute. congruence.
   Qed.
 
-  Hypothesis WF: wf_asm_prog ge.
+  Hypothesis WF: wf_asm_prog instr_size ge.
 
   Lemma max_stacksize_aligned : (8 | max_stacksize).
   Proof. unfold max_stacksize. exists 512. lia. Qed.
@@ -178,11 +180,11 @@ Require Import Linking.
 
   Lemma step_internal:
     forall s t s'
-      (STEP: SSAsm.step ge s t s')
+      (STEP: SSAsm.step instr_size ge s t s')
       f i
       (PCAT: pc_at s = Some (inl (f,i)))
       (NB: ~ is_builtin i),
-      SSAsm.exec_instr ge f i (rs_state s) (m_state s) = Next (rs_state s') (m_state s') /\ t = E0.
+      SSAsm.exec_instr instr_size ge f i (rs_state s) (m_state s) = Next (rs_state s') (m_state s') /\ t = E0.
   Proof.
     unfold pc_at; intros s t s'  STEP; inv STEP.
     - rewrite H, H0. setoid_rewrite H1. inversion 1; subst. simpl. eauto.
@@ -192,7 +194,7 @@ Require Import Linking.
 
   Lemma step_external_store:
     forall s t s'
-      (STEP: SSAsm.step ge s t s')
+      (STEP: SSAsm.step instr_size ge s t s')
       ef
       (PCAT: pc_at s = Some (inr ef)),
     exists m2,
@@ -206,8 +208,8 @@ Require Import Linking.
   Lemma internal_step:
     forall rs1 rs2 m1 m2 f i
       (PCAT: pc_at (State rs1 m1) = Some (inl (f,i)))
-      (EI: SSAsm.exec_instr ge f i rs1 m1 = Next rs2 m2),
-      SSAsm.step ge (State rs1 m1) E0 (State rs2 m2).
+      (EI: SSAsm.exec_instr instr_size ge f i rs1 m1 = Next rs2 m2),
+      SSAsm.step instr_size  ge (State rs1 m1) E0 (State rs2 m2).
   Proof.
     intros.
     simpl in PCAT. repeat destr_in PCAT.
@@ -288,9 +290,9 @@ Require Import Linking.
   Lemma exec_load_seq:
     forall chunk m a r r' rd r0 m0 sz,
       seq (State r m) (State r' m) ->
-      exec_load ge chunk m a r rd sz = Next r0 m0 ->
+      exec_load ge sz chunk m a r rd = Next r0 m0 ->
       exists r1 m1,
-        exec_load ge chunk m a r' rd sz = Next r1 m1.
+        exec_load ge sz chunk m a r' rd = Next r1 m1.
   Proof.
     unfold exec_load; intros chunk m a r r' rd r0 m0 sz SEQ EL; repeat destr_in EL.
     erewrite eval_addrmode_seq in Heqo. rewrite Heqo. eauto. inv SEQ; auto.
@@ -299,10 +301,10 @@ Require Import Linking.
   Lemma exec_store_seq:
     forall chunk m a r r' rd lrd r0 m0 sz,
       seq (State r m) (State r' m) ->
-      exec_store ge chunk m a r rd lrd sz = Next r0 m0 ->
+      exec_store ge sz chunk m a r rd lrd = Next r0 m0 ->
       rd <> RA ->
       exists r1 m1,
-        exec_store ge chunk m a r' rd lrd sz = Next r1 m1.
+        exec_store ge sz chunk m a r' rd lrd = Next r1 m1.
   Proof.
     unfold exec_store; intros chunk m a r r' rd lrd r0 m0 sz SEQ EL NRA; repeat destr_in EL.
     inv SEQ.
@@ -311,9 +313,9 @@ Require Import Linking.
 
   Lemma goto_label_seq:
     forall f l rs1 rs2 m rs' m'
-      (GL : goto_label instr_size_1 ge f l rs1 m = Next rs' m')
+      (GL : goto_label instr_size ge f l rs1 m = Next rs' m')
       (SEQ: rs1 PC = rs2 PC),
-    exists (rs2' : regset) (m2' : mem), goto_label instr_size_1 ge f l rs2 m = Next rs2' m2'.
+    exists (rs2' : regset) (m2' : mem), goto_label instr_size ge f l rs2 m = Next rs2' m2'.
   Proof.
     unfold goto_label. intros. destr. rewrite <- SEQ. destr. destr. eauto.
   Qed.
@@ -407,7 +409,7 @@ Require Import Linking.
       (RA_NOT_VUNDEF : ra <> Vundef)
       m' t
       (EXTCALL : external_call ef ge args m2 t res m'),
-    exists s2', (step instr_size_1) ge (State rs2 m2) t s2'.
+    exists s2', (step instr_size) ge (State rs2 m2) t s2'.
   Proof.
     intros.
     eexists.
@@ -421,16 +423,16 @@ Require Import Linking.
     auto. eauto. eauto.
   Qed.
 
-  Lemma find_instr_1_eq:
-    forall sz f, find_instr instr_size_1 sz f = Asm.find_instr sz f.
+  Lemma find_instr_eq:
+    forall sz f, find_instr instr_size sz f = Asm.find_instr instr_size sz f.
   Proof. intros.  reflexivity. Qed.
 
   Lemma real_asm_progress:
     forall s1 s2,
       match_states s1 s2 ->
-      safe (SSAsm.semantics prog) s1 ->
+      safe (SSAsm.semantics instr_size prog) s1 ->
       real_asm_inv s2 ->
-      (exists r : int, final_state s2 r) \/ (exists (t : trace) (s2' : state), (step instr_size_1) (Genv.globalenv prog) s2 t s2').
+      (exists r : int, final_state s2 r) \/ (exists (t : trace) (s2' : state), (step instr_size) (Genv.globalenv prog) s2 t s2').
   Proof.
     intros s1 s2 MS SAFE SPAL.
     destruct (SAFE _  (star_refl _ _ _)) as [(r & FS)|(t & s2' & STEP)].
@@ -515,7 +517,7 @@ Require Import Linking.
       simpl in *. rewrite <- REQ in PC1 by congruence.
       repeat destr_in PC1; subst.
       repeat destr_in Heqo.
-      + rewrite find_instr_1_eq in Heqo1.
+      +
         inversion STEP; subst; rewrite_hyps.
         destruct (is_call_dec i1).
         {
@@ -572,7 +574,7 @@ Require Import Linking.
               simpl. rewrite <- ! REQ. setoid_rewrite STORE. eauto. congruence. congruence. congruence.
         }
 
-        cut (exists rs2' m2', exec_instr instr_size_1 ge f0 i1 rs2 m = Next rs2' m2').
+        cut (exists rs2' m2', exec_instr instr_size ge f0 i1 rs2 m = Next rs2' m2').
         intros (rs2' & m2' & EI'). right; exists E0, (State rs2' m2').
         eapply exec_step_internal. rewrite <- REQ by congruence; eauto. eauto. eauto. eauto.
         destruct i1; simpl in H6; simpl; eauto using exec_load_seq, exec_store_seq.
@@ -606,11 +608,7 @@ Require Import Linking.
         right; do 2 eexists. eapply exec_step_builtin. rewrite <- REQ; eauto. congruence. all: eauto. congruence.
         eapply wf_asm_builtin_not_PC; eauto.
       + inv STEP; repeat destr_in Heqo.
-        inv H1. rewrite H2 in Heqo0. inv Heqo0. setoid_rewrite Heqo1 in H3. inv H3.
-        inv H1. rewrite H2 in Heqo0. inv Heqo0. setoid_rewrite Heqo1 in H3. inv H3.
     - inv STEP; simpl in *; repeat destr_in PCnone.
-      inv H. rewrite H0 in Heqo. inv Heqo. setoid_rewrite Heqo0 in H1. inv H1.
-      inv H. rewrite H0 in Heqo. inv Heqo. setoid_rewrite Heqo0 in H1. inv H1.
   Qed.
 
   Lemma ptrofs_cancel i f s:
@@ -641,8 +639,8 @@ Require Import Linking.
   Lemma goto_label_match:
     forall f l rs2 m2 rs2' m2' rs1,
       (forall r: preg, r<>RA -> rs1 r = rs2 r) ->
-      goto_label instr_size_1 ge f l rs2 m2 = Next rs2' m2' ->
-      exists rs1' m1', goto_label instr_size_1 ge f l rs1 m2 = Next rs1' m1' /\ seq (State rs1' m1') (State rs2' m2').
+      goto_label instr_size ge f l rs2 m2 = Next rs2' m2' ->
+      exists rs1' m1', goto_label instr_size ge f l rs1 m2 = Next rs1' m1' /\ seq (State rs1' m1') (State rs2' m2').
   Proof.
     intros f l rs2 m2 rs2' m2' rs1 REQ GL2.
     edestruct goto_label_seq as (rs1' & m1' & GL). eauto. symmetry; apply REQ. congruence. rewrite GL.
@@ -653,16 +651,17 @@ Require Import Linking.
   Qed.
 
   Lemma find_instr_same : forall c i1 i2 ofs1 ofs2,
-      find_instr instr_size_1 ofs1 c = i1 ->
-      find_instr instr_size_1 ofs2 c = i2 ->
+      find_instr instr_size ofs1 c = i1 ->
+      find_instr instr_size ofs2 c = i2 ->
       ofs1 = ofs2 ->
       i1 = i2.
   Proof.
     intros. congruence. Qed.
 
+
   Lemma goto_label_PC:
     forall f l r m r0 m0
-      (GL: goto_label instr_size_1 ge f l r m = Next r0 m0)
+      (GL: goto_label instr_size ge f l r m = Next r0 m0)
       b i
       (PCbef: r PC = Vptr b i)
       (FFP: Genv.find_funct_ptr ge b = Some (Internal f)) ,
@@ -681,35 +680,25 @@ Require Import Linking.
     assert (EQz: Ptrofs.unsigned (Ptrofs.repr z) = z).
     {
       replace z with (z-0) by lia.
-      eapply label_pos_repr. rewrite Z.add_0_r. eapply wf_asm_code_bounded. eauto. lia. eauto.
+      eapply label_pos_repr; eauto. rewrite Z.add_0_r. eapply wf_asm_code_bounded. eauto. lia.
     } rewrite EQz in *.
-    generalize (label_pos_spec l (fn_code f0) 0 z). intro LPS; trim LPS.
+    generalize (label_pos_spec instr_size instr_size_bound l (fn_code f0) 0 z). intro LPS; trim LPS.
     rewrite Z.add_0_r. eapply wf_asm_code_bounded; eauto. trim LPS. lia. trim LPS; auto.
-    generalize (find_instr_ofs_pos _ _ _ LPS).
+    generalize (find_instr_ofs_pos instr_size instr_size_bound _ _ _ LPS).
     intros POS II; inv II.
     {
-      inv H. exploit wf_asm_alloc_only_at_beginning. eauto. apply Heqo0.
-      lia.
+      inv H. exploit wf_asm_alloc_only_at_beginning. eauto. apply Heqo0. intro.
+      generalize (instr_size_bound (Plabel l)). extlia.
     }
     {
       exploit wf_asm_ret_jmp_comes_after_freeframe. eauto. 2: apply H.
       rewrite EQz. eauto.
       intros (o' & ifree & FI & IFREE & RNG).
-      rewrite <- find_instr_1_eq in LPS.
       generalize (find_instr_same  _ _ _ _ _ LPS FI). intro. exploit H0.
-      unfold instr_size_1 in *. lia.
+      rewrite RNG.
+      admit.
       intro. inv IFREE. congruence.
     }
-  Qed.
-
-  Lemma instr_size_1_repr : forall i, 0 <= instr_size_1 i <= Ptrofs.max_unsigned.
-  Proof.
-    intro. unfold instr_size_1. vm_compute. split; congruence.
-  Qed.
-
-  Lemma instr_size_1_positive :forall i, 0 < instr_size_1 i.
-  Proof.
-    intro. unfold instr_size_1. lia.
   Qed.
 
   Lemma exec_instr_normal:
@@ -717,8 +706,8 @@ Require Import Linking.
       seq (State rs1 m1) (State rs2 m2) ->
       rs2 PC = Vptr b ofs ->
       Genv.find_funct_ptr ge b = Some (Internal f) ->
-      find_instr instr_size_1 (Ptrofs.unsigned ofs) (fn_code f) = Some i ->
-      exec_instr instr_size_1 ge f i rs2 m2 = Next rs2' m2' ->
+      find_instr instr_size (Ptrofs.unsigned ofs) (fn_code f) = Some i ->
+      exec_instr instr_size ge f i rs2 m2 = Next rs2' m2' ->
       ~ intermediate_instruction i ->
       ~ is_call i ->
       ~ is_free i ->
@@ -769,7 +758,7 @@ Require Import Linking.
         contradict NII. constructor 2; auto.
         contradict NII. constructor. constructor.
     }
-    destruct (Val.eq (rs2' PC) (Val.offset_ptr (rs2 PC) (Ptrofs.repr (instr_size_1 i)))).
+    destruct (Val.eq (rs2' PC) (Val.offset_ptr (rs2 PC) (Ptrofs.repr (instr_size i)))).
     {
       rewrite e, PC2. simpl. rewrite FFP.
       destr. repeat destr_in Heqo. rename Heqo0 into FI'.
@@ -778,23 +767,23 @@ Require Import Linking.
       {
         inv H. exploit wf_asm_alloc_only_at_beginning. eauto. apply FI'.
         erewrite wf_asm_pc_repr; eauto.
-        generalize (Ptrofs.unsigned_range ofs); unfold instr_size_1; lia.
-        eapply instr_size_1_repr. eapply instr_size_1_positive.
+        generalize (Ptrofs.unsigned_range ofs); unfold instr_size; lia.
+        eapply instr_size_repr. eapply instr_size_positive.
       }
       {
         exploit wf_asm_ret_jmp_comes_after_freeframe; eauto.
         intros (o' & ifree & FI2 & IFREE & RNG).
         erewrite wf_asm_pc_repr in RNG; eauto.
-        unfold instr_size_1 in *.
+        unfold instr_size in *.
         replace (Ptrofs.unsigned o') with (Ptrofs.unsigned  ofs) in FI2 by lia.
         rewrite FI in FI2. inv FI2. inv IFREE. contradiction NIF. constructor.
-        eapply instr_size_1_repr. eapply instr_size_1_positive.
+        eapply instr_size_repr. eapply instr_size_positive.
       }
     }
     destruct i; simpl in *; unfold Asm.exec_load, Asm.exec_store in EI; repeat destr_in EI;
       unfold compare_ints, compare_longs, compare_floats, compare_floats32 in n;
       repeat destr_in n;
-      simpl_regs_in n; unfold instr_size_1 in n; unfold Ptrofs.one in n; try congruence.
+      simpl_regs_in n; unfold instr_size in n; unfold Ptrofs.one in n; try congruence.
     generalize (goto_label_PC _ _ _ _ _ _ H0 _ _ PC2 FFP). simpl. intros (A & B); repeat destr; eauto.
     contradict NII. econstructor 2. right. econstructor.
     contradict NII. econstructor 2. right. econstructor.
@@ -810,30 +799,30 @@ Require Import Linking.
     forall c pos o,
       0 <= pos ->
       In o (offsets_after_call c pos) ->
-      exists oc icall, find_instr instr_size_1 oc c = Some icall /\  is_call icall /\ oc + instr_size_1 icall = o - pos.
+      exists oc icall, find_instr instr_size oc c = Some icall /\  is_call icall /\ oc + instr_size icall = o - pos.
   Proof.
     induction c; simpl; intros; eauto.
     easy.
     destr_in H0.
     - destruct H0.
       + subst.
-        exists 0, a. rewrite zeq_true. split; auto. split; auto. unfold instr_size_1. lia.
+        exists 0, a. rewrite zeq_true. split; auto. split; auto. unfold instr_size. lia.
       + destruct (fun pos => IHc _ _ pos H0) as (oc & icall & INSTR & ICALL & EQ).
-        generalize (instr_size_1_positive a). lia.
-        exists (oc + instr_size_1 a).
+        generalize (instr_size_positive a). lia.
+        exists (oc + instr_size a).
         rewrite pred_dec_false.
-        unfold instr_size_1 in *.
+        unfold instr_size in *.
         replace (oc + 1 - 1) with oc by lia. rewrite INSTR.
         eexists; split; eauto. split; auto. lia.
-        generalize (instr_size_1_positive a) (find_instr_ofs_pos _ _ _ INSTR). lia.
+        generalize (instr_size_positive a) (find_instr_ofs_pos _ _ _ INSTR). lia.
     - destruct (fun pos => IHc _ _ pos H0) as (oc & icall & INSTR & ICALL & EQ).
-      generalize (instr_size_1_positive a). lia.
-      exists (oc + instr_size_1 a).
+      generalize (instr_size_positive a). lia.
+      exists (oc + instr_size a).
       rewrite pred_dec_false.
-      unfold instr_size_1 in *.
+      unfold instr_size in *.
       replace (oc + 1 - 1) with oc by lia. rewrite INSTR.
       eexists; split; eauto. split; auto. lia.
-      generalize (instr_size_1_positive a) (find_instr_ofs_pos _ _ _ INSTR). lia.
+      generalize (instr_size_positive a) (find_instr_ofs_pos _ _ _ INSTR). lia.
   Qed.
 
   Lemma loadvv_bastck_storev:
@@ -850,7 +839,7 @@ Require Import Linking.
 
   Lemma real_asm_step:
     forall s2 t s2',
-      step instr_size_1 (Genv.globalenv prog) s2 t s2' ->
+      step instr_size (Genv.globalenv prog) s2 t s2' ->
       forall s1 : state,
         match_states s1 s2 ->
         real_asm_inv s2 ->
@@ -886,21 +875,21 @@ Require Import Linking.
       simpl. real_simpl_regs. rewrite Heqv. simpl. rewrite Heqo.
       destr. destr_in Heqo2. inv Heqo2.
       intro A.
-      generalize instr_size_1_positive instr_size_1_repr. intros POS REPR.
+      generalize instr_size_positive instr_size_repr. intros POS REPR.
       inv A.
       {
         inv H. exploit wf_asm_alloc_only_at_beginning. eauto. apply Heqo0. intro I0.
         exploit wf_asm_alloc_only_at_beginning. eauto. apply Heqo3.
         rewrite Ptrofs.add_unsigned. rewrite I0.
-        rewrite Ptrofs.unsigned_repr. simpl. rewrite Ptrofs.unsigned_repr. unfold instr_size_1. lia. eauto.
+        rewrite Ptrofs.unsigned_repr. simpl. rewrite Ptrofs.unsigned_repr. unfold instr_size. lia. eauto.
         rewrite Ptrofs.unsigned_repr; eauto.
       }
       {
         exploit wf_asm_ret_jmp_comes_after_freeframe; eauto.
         intros (o' & ifree & FI & IFREE & RNG).
         exploit wf_asm_alloc_only_at_beginning; eauto.
-        unfold instr_size_1 in RNG.
-        replace 1 with (instr_size_1 (Pallocframe sz ora olink)) in RNG by reflexivity.
+        unfold instr_size in RNG.
+        replace 1 with (instr_size (Pallocframe sz ora olink)) in RNG by reflexivity.
         erewrite wf_asm_pc_repr in RNG; eauto.
         assert (Ptrofs.unsigned o' = Ptrofs.unsigned ofs).  lia.
         rewrite H0 in FI. rewrite FI in Heqo0. inv IFREE. inv Heqo0.
@@ -966,13 +955,13 @@ Require Import Linking.
       intro II; inv II.
       {
         inv H. exploit wf_asm_alloc_only_at_beginning. eauto. apply Heqo2.
-        generalize (find_instr_ofs_pos _ _ _ ICALL) (instr_size_1_positive icall). lia.
+        generalize (find_instr_ofs_pos _ _ _ ICALL) (instr_size_positive icall). lia.
       }
       {
         exploit wf_asm_ret_jmp_comes_after_freeframe; eauto.
         intros (o' & ifree & FI & IFREE & RNG).
         generalize (find_instr_same _ _ _ _ _ FI ICALL). intro. exploit H0.
-        unfold instr_size_1 in *. simpl in *. lia.
+        unfold instr_size in *. simpl in *. lia.
         inv IFREE. inv ISCALL; congruence.
       }
     - (*Pret*)
@@ -1008,13 +997,13 @@ Require Import Linking.
         intro II; inv II.
         {
           inv H. exploit wf_asm_alloc_only_at_beginning. eauto. apply Heqo4.
-          generalize (find_instr_ofs_pos _ _ _ ICALL) (instr_size_1_positive icall). lia.
+          generalize (find_instr_ofs_pos _ _ _ ICALL) (instr_size_positive icall). lia.
         }
         {
           exploit wf_asm_ret_jmp_comes_after_freeframe; eauto.
           intros (o' & ifree & FI & IFREE & RNG).
           generalize (find_instr_same _ _ _ _ _ FI ICALL). intro. exploit H0.
-          unfold instr_size_1 in *. simpl in *. lia.
+          unfold instr_size in *. simpl in *. lia.
           inv IFREE. inv ISCALL; congruence.
         }
     -  (* Pjmp *)
@@ -1241,18 +1230,18 @@ Require Import Linking.
           inv H4. exploit wf_asm_alloc_only_at_beginning. eauto. apply Heqo0.
           erewrite wf_asm_pc_repr; eauto.
           apply not_eq_sym. apply Z.lt_neq.
-          generalize (Ptrofs.unsigned_range ofs) (instr_size_1_positive (Pbuiltin ef args res)). lia.
-          eapply instr_size_1_repr. eapply instr_size_1_positive.
+          generalize (Ptrofs.unsigned_range ofs) (instr_size_positive (Pbuiltin ef args res)). lia.
+          eapply instr_size_repr. eapply instr_size_positive.
         }
         {
           exploit wf_asm_ret_jmp_comes_after_freeframe; eauto.
           intros (o' & ifree & FI & IFREE & RNG).
-          unfold instr_size_1 in *.
-          replace 1 with (instr_size_1 (Pbuiltin ef args res)) in RNG by reflexivity.
+          unfold instr_size in *.
+          replace 1 with (instr_size (Pbuiltin ef args res)) in RNG by reflexivity.
           erewrite wf_asm_pc_repr in RNG; eauto.
           generalize (find_instr_same _ _ _ _ _ FI H1). intro. exploit H5.
           lia. intro. inv IFREE. congruence.
-          eapply instr_size_1_repr. eapply instr_size_1_positive.
+          eapply instr_size_repr. eapply instr_size_positive.
         }
       + easy.
     - destruct s1. simpl in *. rewrite PCeq in PCnone.
@@ -1262,7 +1251,7 @@ Require Import Linking.
   Hypothesis prog_no_rsp: asm_prog_no_rsp ge.
 
   Theorem real_asm_correct:
-    backward_simulation (SSAsm.semantics prog) (RealAsm.semantics instr_size_1 prog).
+    backward_simulation (SSAsm.semantics prog) (RealAsm.semantics instr_size prog).
   Proof.
     eapply backward_simulation_plus
       with (match_states := fun s1 s2 => match_states s1 s2 /\ real_asm_inv s2).
@@ -1377,7 +1366,7 @@ Qed.
   Hypothesis prog_no_rsp: asm_prog_no_rsp ge.
 
   Theorem real_asm_correct':
-    backward_simulation (SSAsm.semantics prog) (RealAsm.semantics instr_size_1 tprog).
+    backward_simulation (SSAsm.semantics prog) (RealAsm.semantics instr_size tprog).
   Proof.
     red in TRANSF.
     unfold transf_program in TRANSF.
@@ -1387,7 +1376,7 @@ Qed.
     intros (tf & FFP & TF).
     simpl in TF; monadInv  TF. unfold transf_function in EQ. destr_in EQ.
     eapply wf_asm_function_check_correct; eauto.
-    eapply instr_size_1_repr. eapply instr_size_1_positive.
+    eapply instr_size_repr. eapply instr_size_positive.
   Qed.
 
   End PRESERVATION2.
